cogent/examples/wa_connect/WordArray_CorresProof_Asm.thy
@@ -10,28 +10,25 @@ context WordArray begin
 
 section "Level 0 Assumptions"
 
-lemma val_mono_prog_wa_length:
-  "\<And>v v'.
-       \<lbrakk>val_wa_length (val.rename_val rename' (val.monoval v)) v'; val.proc_env_matches \<xi>\<^sub>v \<Xi>'; proc_ctx_wellformed \<Xi>'\<rbrakk>
-       \<Longrightarrow> v' = val.rename_val rename' (val.monoval v') \<and> val_wa_length v v'"
+lemma val_wa_length_rename_monoexpr_correct:
+  "\<lbrakk>val_wa_length (val.rename_val rename' (val.monoval v)) v'; val.proc_env_matches \<xi>\<^sub>v \<Xi>'; proc_ctx_wellformed \<Xi>'\<rbrakk>
+    \<Longrightarrow> v' = val.rename_val rename' (val.monoval v') \<and> val_wa_length v v'"
   apply (clarsimp simp: val_wa_length_def)
   apply (case_tac v; clarsimp)
   done
 
-lemma val_mono_prog_wa_get:
-  "\<And>v v'.
-       \<lbrakk>val_wa_get (val.rename_val rename' (val.monoval v)) v'; val.proc_env_matches \<xi>\<^sub>v \<Xi>'; proc_ctx_wellformed \<Xi>'\<rbrakk>
-       \<Longrightarrow> v' = val.rename_val rename' (val.monoval v') \<and> val_wa_get v v'"
+lemma val_wa_get_rename_monoexpr_correct:
+  "\<lbrakk>val_wa_get (val.rename_val rename' (val.monoval v)) v'; val.proc_env_matches \<xi>\<^sub>v \<Xi>'; proc_ctx_wellformed \<Xi>'\<rbrakk>
+    \<Longrightarrow> v' = val.rename_val rename' (val.monoval v') \<and> val_wa_get v v'"
   apply (clarsimp simp: val_wa_get_def)
   apply (case_tac v; clarsimp)
   apply (case_tac z; clarsimp)
   apply (case_tac za; clarsimp)
   done
 
-lemma val_mono_prog_wa_put2:
-  "\<And>v v'.
-       \<lbrakk>val_wa_put2 (val.rename_val rename' (val.monoval v)) v'; val.proc_env_matches \<xi>\<^sub>v \<Xi>'; proc_ctx_wellformed \<Xi>'\<rbrakk>
-       \<Longrightarrow> v' = val.rename_val rename' (val.monoval v') \<and> val_wa_put2 v v'"
+lemma val_wa_put2_rename_monoexpr_correct:
+  "\<lbrakk>val_wa_put2 (val.rename_val rename' (val.monoval v)) v'; val.proc_env_matches \<xi>\<^sub>v \<Xi>'; proc_ctx_wellformed \<Xi>'\<rbrakk>
+    \<Longrightarrow> v' = val.rename_val rename' (val.monoval v') \<and> val_wa_put2 v v'"
   apply (clarsimp simp: val_wa_put2_def)
   apply (case_tac v; clarsimp)
   apply (case_tac z; clarsimp)
@@ -48,23 +45,23 @@ lemma value_sem_rename_mono_prog_rename_\<Xi>_\<xi>m_\<xi>p:
    apply (subst (asm) rename_def)
    apply (subst (asm) assoc_lookup.simps)+
    apply (clarsimp split: if_split_asm)
-  apply (clarsimp simp: val_mono_prog_wa_length)
+  apply (clarsimp simp: val_wa_length_rename_monoexpr_correct)
   apply (rule conjI)
    apply clarsimp
    apply (rule_tac x = v' in exI)
    apply (subst (asm) rename_def)
    apply (subst (asm) assoc_lookup.simps)+
    apply (clarsimp split: if_split_asm)
-  apply (clarsimp simp: val_mono_prog_wa_get)
+  apply (clarsimp simp: val_wa_get_rename_monoexpr_correct)
   apply clarsimp
   apply (rule_tac x = v' in exI)
   apply (subst (asm) rename_def)
   apply (subst (asm) assoc_lookup.simps)+
   apply (clarsimp split: if_split_asm)
-  apply (clarsimp simp: val_mono_prog_wa_put2)
+  apply (clarsimp simp: val_wa_put2_rename_monoexpr_correct)
   done
 
-lemma val_proc_env_matches_wa_get:
+lemma val_wa_get_preservation:
   "\<lbrakk>val.vval_typing \<Xi>' v (TRecord [(a, TCon ''WordArray'' [t] (Boxed ReadOnly ptrl), Present),
       (b, TPrim (Num U32), Present)] Unboxed); val_wa_get v v'\<rbrakk>
     \<Longrightarrow> val.vval_typing \<Xi>' v' t"
@@ -75,14 +72,14 @@ lemma val_proc_env_matches_wa_get:
   apply (rule val.v_t_prim'; clarsimp)
   done
 
-lemma val_proc_env_matches_wa_length:
+lemma val_wa_length_preservation:
   "\<lbrakk>val.vval_typing \<Xi>' v (TCon ''WordArray'' [t] (Boxed ReadOnly ptrl)); val_wa_length v v'\<rbrakk>
     \<Longrightarrow> val.vval_typing \<Xi>' v' (TPrim (Num U32))"
   apply (clarsimp simp:  val_wa_length_def)
   apply (rule val.v_t_prim'; clarsimp)
   done
 
-lemma val_proc_env_matches_wa_put2:
+lemma val_wa_put2_preservation:
   "\<lbrakk>val.vval_typing \<Xi>' v (TRecord [(a, TCon ''WordArray'' [t] (Boxed Writable ptrl), Present),
       (b', TPrim (Num U32), Present), (c, t, Present)] Unboxed); val_wa_put2 v v'\<rbrakk>
     \<Longrightarrow> val.vval_typing \<Xi>' v' (TCon ''WordArray'' [t] (Boxed Writable ptrl))"
@@ -102,11 +99,11 @@ lemma val_proc_env_matches_\<xi>m_\<Xi>:
   apply (subst (asm) assoc_lookup.simps)+
   apply (clarsimp split: if_split_asm)
     apply (clarsimp simp: wordarray_get_0_type_def abbreviatedType3_def)
-    apply (drule val_proc_env_matches_wa_get; simp?)
+    apply (drule val_wa_get_preservation; simp?)
    apply (clarsimp simp: wordarray_length_0_type_def)
-  apply (drule val_proc_env_matches_wa_length; simp?)
+  apply (drule val_wa_length_preservation; simp?)
   apply (clarsimp simp: wordarray_put2_0_type_def abbreviatedType2_def)
-  apply (drule val_proc_env_matches_wa_put2; simp?)
+  apply (drule val_wa_put2_preservation; simp?)
   done
 
 lemma wa_get_upd_val:
@@ -264,7 +261,7 @@ lemma proc_env_u_v_matches_\<xi>0_\<xi>m_\<Xi>:
   apply (drule wa_put2_upd_val; simp)
   done
 
-lemma wa_get_uval_typing_frame:
+lemma upd_wa_get_preservation:
   "\<lbrakk>upd.uval_typing \<Xi>' \<sigma> v (TRecord [(a, TCon ''WordArray'' [t] (Boxed ReadOnly ptrl), Present),
       (b, TPrim (Num U32), Present)] Unboxed) r w; upd_wa_get_0 (\<sigma>, v) (\<sigma>', v')\<rbrakk>
     \<Longrightarrow> \<exists>r' w'. upd.uval_typing \<Xi>' \<sigma>' v' t r' w' \<and> r' \<subseteq> r \<and> frame \<sigma> w \<sigma>' w'"
@@ -287,7 +284,7 @@ lemma wa_get_uval_typing_frame:
   apply (case_tac ta; clarsimp intro!: upd.u_t_prim')
   done
 
-lemma wa_length_uval_typing_frame:
+lemma upd_wa_length_preservation:
   "\<lbrakk>upd.uval_typing \<Xi>' \<sigma> v (TCon ''WordArray'' [t] (Boxed ReadOnly ptrl)) r w;
     upd_wa_length_0 (\<sigma>, v) (\<sigma>', v')\<rbrakk>
     \<Longrightarrow> \<exists>r' w'. upd.uval_typing \<Xi>' \<sigma>' v' (TPrim (Num U32)) r' w' \<and> r' \<subseteq> r \<and> frame \<sigma> w \<sigma>' w'"
@@ -299,7 +296,7 @@ lemma wa_length_uval_typing_frame:
 
 inductive_cases upd_u_t_prim_tE: "upd.uval_typing \<Xi>' \<sigma> u (TPrim l) r w"
 
-lemma wa_put2_uval_typing_frame:
+lemma upd_wa_put2_preservation:
   "\<lbrakk>upd.uval_typing \<Xi>' \<sigma> v (TRecord [(a, TCon ''WordArray'' [t] (Boxed Writable ptrl), Present),
       (b, TPrim (Num U32), Present), (c, t, Present)] Unboxed) r w; upd_wa_put2_0 (\<sigma>, v) (\<sigma>', v')\<rbrakk>
     \<Longrightarrow> \<exists>r' w'. upd.uval_typing \<Xi>' \<sigma>' v' (TCon ''WordArray'' [t] (Boxed Writable ptrl)) r' w' \<and>
@@ -356,11 +353,11 @@ lemma upd_proc_env_matches_ptrs_\<xi>0_\<Xi>:
   apply (subst (asm) assoc_lookup.simps)+
   apply (clarsimp split: if_split_asm)
     apply (clarsimp simp: wordarray_get_0_type_def abbreviatedType3_def)
-    apply (drule wa_get_uval_typing_frame; simp?)
+    apply (drule upd_wa_get_preservation; simp?)
    apply (clarsimp simp: wordarray_length_0_type_def)
-  apply (drule wa_length_uval_typing_frame; simp)
+  apply (drule upd_wa_length_preservation; simp)
   apply (clarsimp simp: wordarray_put2_0_type_def abbreviatedType2_def)
-  apply (drule wa_put2_uval_typing_frame; simp)
+  apply (drule upd_wa_put2_preservation; simp)
   done
 
 lemma proc_ctx_wellformed_\<Xi>:
@@ -378,80 +375,191 @@ lemma proc_ctx_wellformed_\<Xi>:
 
 section "Level 1 Assumptions"
 
-lemma wordarray_fold_no_break_uval_typing_frame:
+lemma upd_wa_foldnb_bod_preservation:
+  "\<lbrakk>proc_ctx_wellformed \<Xi>'; upd.proc_env_matches_ptrs \<xi>\<^sub>u \<Xi>';
+    upd_wa_foldnb_bod \<xi>\<^sub>u \<sigma> p frm to f acc obsv (rb \<union> rc) (\<sigma>', res);
+    \<sigma> p = option.Some (UAbstract (UWA t len arr)); 
+    wa_abs_typing_u (UWA t len arr) ''WordArray'' [t] (Boxed ReadOnly ptrl) ra wa \<sigma>;
+    upd.uval_typing \<Xi>' \<sigma> acc u rb wb; upd.uval_typing \<Xi>' \<sigma> obsv v rc {};  wb \<inter> rc = {};
+    \<Xi>', [], [option.Some (TRecord [
+      (b0, t, Present), (b1, u, Present), (b2, v, Present)] Unboxed)] \<turnstile> (App f (Var 0)) : u;
+    distinct [b0, b1, b2]\<rbrakk>
+    \<Longrightarrow> \<exists>r' w'. upd.uval_typing \<Xi>' \<sigma>' res u r' w' \<and> r' \<subseteq> (ra \<union> rb \<union> rc) \<and> frame \<sigma> wb \<sigma>' w'"
+  apply (induct to arbitrary: \<sigma>' res)
+   apply (erule upd_wa_foldnb_bod.elims; clarsimp)
+   apply (rule_tac x = rb in exI)
+   apply (rule_tac x = wb in exI)
+   apply (clarsimp simp: frame_def)
+  apply (case_tac "len < 1 + to")
+   apply (drule upd_wa_foldnb_bod_back_step'; simp?)
+  apply (case_tac "1 + to \<le> frm")
+   apply (frule_tac y = "1 + to" and x = frm in leD)
+   apply (erule upd_wa_foldnb_bod.elims; clarsimp)
+   apply (rule_tac x = rb in exI)
+   apply (rule_tac x = wb in exI)
+   apply (clarsimp simp: frame_def)
+  apply (case_tac "frm = to")
+   apply (clarsimp simp: not_le not_less)
+   apply (frule_tac z = len in less_le_trans, simp)
+   apply (erule upd_wa_foldnb_bod.elims; clarsimp)
+   apply (erule upd_wa_foldnb_bod.elims; clarsimp simp: add.commute)
+   apply (drule_tac ?\<Gamma> = "[option.Some (TRecord [(b0, TPrim (Num ta), Present), (b1, u, Present),
+    (b2, v, Present)] Unboxed)]" and r = "rb \<union> rc" and  w = wb and \<tau> = u in upd.preservation_mono(1); simp?)
+    apply (rule upd.matches_ptrs_some[where ts = "[]" and r' = "{}" and w' = "{}", simplified])
+     apply (rule upd.u_t_struct; simp?)
+     apply (rule upd.u_t_r_cons1[where r = "{}" and w = "{}", simplified])
+       apply (clarsimp simp: wa_abs_typing_u_def)
+       apply (erule_tac x = frm in allE; clarsimp)+
+       apply (rule upd.u_t_prim'; clarsimp)
+      apply (rule upd.u_t_r_cons1[where r' = rc and w' = "{}", simplified]; simp?)
+       apply (rule upd.u_t_r_cons1[where r' = "{}" and w' = "{}", simplified]; simp?)
+        apply (rule upd.u_t_r_empty)
+       apply (drule_tac v = obsv in upd.type_repr_uval_repr(1); simp)
+      apply (drule_tac v = acc in upd.type_repr_uval_repr(1); simp)
+     apply (clarsimp simp: wa_abs_typing_u_def)
+     apply (erule_tac x = frm in allE; clarsimp)+
+    apply (rule upd.matches_ptrs_empty[where \<tau>s = "[]", simplified])
+   apply blast
+  apply (clarsimp simp: wa_abs_typing_u_def)
+  apply (case_tac t; clarsimp)
+  apply (case_tac x5; clarsimp)
+  apply (drule upd_wa_foldnb_bod_back_step; simp?)
+    apply (metis (no_types, hide_lams) word_le_less_eq word_zero_le)
+   apply (metis (full_types) add.commute inc_le word_le_less_eq word_not_le)
+  apply clarsimp
+  apply (drule_tac x = \<sigma>'' in meta_spec)
+  apply (drule_tac x = r'' in meta_spec)
+  apply clarsimp
+  apply (erule_tac x = to in allE; clarsimp)+
+  apply (erule impE)
+   apply (cut_tac x = to in word_overflow)
+   apply (erule disjE; clarsimp simp: add.commute)
+   apply auto[1]
+  apply clarsimp
+  apply (drule_tac ?\<Gamma> = "[option.Some (TRecord [(b0, TPrim (Num x1), Present), (b1, u, Present),
+    (b2, v, Present)] Unboxed)]" and r = "r' \<union> rc" and  w = w' and \<tau> = u in upd.preservation_mono(1); simp?)
+   apply (rule upd.matches_ptrs_some[where ts = "[]" and r' = "{}" and w' = "{}", simplified])
+    apply (rule upd.u_t_struct; simp?)
+    apply (rule upd.u_t_r_cons1[where r = "{}" and w = "{}", simplified])
+      apply (rule upd.u_t_prim'; clarsimp)
+     apply (rule upd.u_t_r_cons1[where r' = rc and w' = "{}", simplified]; simp?)
+       apply (rule upd.u_t_r_cons1[where r' = "{}" and w' = "{}", simplified]; simp?)
+         apply (rule upd.uval_typing_frame(1); simp?)
+         apply (rule disjointI)
+         apply (clarsimp simp: frame_def)
+         apply (erule_tac x = y in allE; clarsimp)
+         apply (drule_tac x = y in orthD1; simp)
+        apply (rule upd.u_t_r_empty)
+       apply (drule_tac v = obsv in upd.type_repr_uval_repr(1); simp)
+      apply (rule disjointI)
+      apply (thin_tac "frame _ _ _ _")
+      apply (clarsimp simp: frame_def)
+      apply (erule_tac x = y in allE; clarsimp)+
+      apply (drule_tac x = y in orthD2; simp)
+      apply (drule_tac u = obsv and p = y in upd.uval_typing_valid(1)[rotated 1]; simp)
+     apply (drule_tac v = r'' in upd.type_repr_uval_repr(1); simp)
+    apply clarsimp
+   apply (rule upd.matches_ptrs_empty[where \<tau>s = "[]", simplified])
+  apply clarsimp
+  apply (thin_tac "frame _ _ _ _")
+  apply (rule_tac x = r'a in exI)
+  apply (rule_tac x = w'a in exI)
+  apply clarsimp
+  apply (rule conjI, blast)
+  apply (rule upd.frame_trans; simp)
+  done
+
+lemma upd_wa_foldnb_0_preservation:
   "\<And>K a b \<sigma> \<sigma>' \<tau>s v v' r w.
    \<lbrakk>list_all2 (kinding []) \<tau>s K; wordarray_fold_no_break_0_type = (K, a, b);
     upd.uval_typing \<Xi> \<sigma> v (instantiate \<tau>s a) r w; upd_wa_foldnb_0 (\<sigma>, v) (\<sigma>', v')\<rbrakk>
     \<Longrightarrow> \<exists>r' w'. upd.uval_typing \<Xi> \<sigma>' v' (instantiate \<tau>s b) r' w' \<and> r' \<subseteq> r \<and> frame \<sigma> w \<sigma>' w'"
   apply (clarsimp simp: wordarray_fold_no_break_0_type_def upd_wa_foldnb_0_def)
-  apply (rule_tac x = "{}" in exI)
-  apply (rule_tac x = w in exI)
-  apply (clarsimp simp: frame_def)
   apply (erule upd.u_t_recE; clarsimp)
   apply (erule upd.u_t_r_consE; clarsimp)
+  apply (erule upd.u_t_r_consE; simp)
+  apply (erule conjE)+
+  apply (drule_tac t = "type_repr _" in sym; clarsimp)
+  apply (erule upd.u_t_r_consE; simp)
+  apply (erule conjE)+
+  apply (drule_tac t = "type_repr _" in sym; clarsimp)
+  apply (erule upd.u_t_r_consE; simp)
+  apply (erule conjE)+
+  apply (drule_tac t = "type_repr _" in sym; clarsimp)
+  apply (erule upd.u_t_r_consE; simp)
+  apply (erule conjE)+
+  apply (drule_tac t = "type_repr _" in sym; clarsimp)
+  apply (erule upd.u_t_r_consE; simp)
+  apply (erule conjE)+
+  apply clarsimp
+  apply (erule upd.u_t_r_emptyE; clarsimp)
   apply (erule upd.u_t_p_absE; clarsimp)
-  apply (erule upd.u_t_r_consE; simp)
-  apply (erule conjE)+
-  apply (subst (asm) type_repr.simps[symmetric])+
-  apply clarsimp
-  apply (erule upd.u_t_r_consE; simp)
-  apply (erule conjE)+
-  apply (subst (asm) type_repr.simps[symmetric])+
-  apply clarsimp
-  apply (erule upd.u_t_r_consE; simp)
-  apply (erule conjE)+
-  apply (subst (asm) type_repr.simps[symmetric])+
-  apply clarsimp
-  apply (erule upd.u_t_r_consE; simp)
-  apply (erule conjE)+
-  apply (subst (asm) type_repr.simps[symmetric])+
-  apply clarsimp
-  apply (erule upd.u_t_r_consE; simp)
-  apply (erule conjE)+
-  apply clarsimp
-  apply (erule upd.u_t_r_emptyE)
   apply (erule upd.u_t_primE)+
-  apply (subst (asm) lit_type.simps)+
+  apply (drule_tac t = "lit_type _" in sym)+
   apply clarsimp
-  apply (erule upd.u_t_unitE)
-  apply clarsimp
-  apply (case_tac xa; clarsimp)
-   apply (erule upd.u_t_funE'; clarsimp)
-   apply (rule upd.u_t_prim[where l = "LU32 _", simplified])
+  apply (erule upd.u_t_unitE; clarsimp)
+  apply (case_tac xa; clarsimp simp: abbreviatedType1_def)
+  apply (erule upd.u_t_functionE; clarsimp)
+   apply (drule_tac ra = rg in upd_wa_foldnb_bod_preservation[OF proc_ctx_wellformed_\<Xi> 
+        upd_proc_env_matches_ptrs_\<xi>0_\<Xi>, where rb = "{}" and rc = "{}" and 
+        ptrl = undefined and wa = "{}" and wb = "{}", simplified]; simp?; clarsimp?)
+     apply (rule upd.u_t_prim'; clarsimp)
+    apply (rule upd.u_t_unit)
+   apply blast
   apply (erule upd.u_t_afunE; clarsimp)
-  apply (rule upd.u_t_prim[where l = "LU32 _", simplified])
+  apply (drule_tac ra = rg in upd_wa_foldnb_bod_preservation[OF proc_ctx_wellformed_\<Xi> 
+        upd_proc_env_matches_ptrs_\<xi>0_\<Xi>, where rb = "{}" and rc = "{}" and 
+        ptrl = undefined and wa = "{}" and wb = "{}", simplified]; simp?; clarsimp?)
+    apply (rule upd.u_t_prim'; clarsimp)
+   apply (rule upd.u_t_unit)
+  apply blast
   done
 
 inductive_cases v_t_prim_tE : "val.vval_typing \<Xi>' v (TPrim l)"
 
-lemma lit_type_ex_32:
+lemma lit_type_ex:
+  "lit_type l = Bool \<Longrightarrow> \<exists>v. l = LBool v"
+  "lit_type l = Num U8 \<Longrightarrow> \<exists>v. l = LU8 v"
+  "lit_type l = Num U16 \<Longrightarrow> \<exists>v. l = LU16 v"
   "lit_type l = Num U32 \<Longrightarrow> \<exists>v. l = LU32 v"
-  apply (induct l; clarsimp)
+  "lit_type l = Num U64 \<Longrightarrow> \<exists>v. l = LU64 v"
+  apply (induct l; clarsimp)+
   done
+
+lemma 
+  "\<lbrakk>val.proc_env_matches \<xi>\<^sub>m \<Xi>'; proc_ctx_wellformed \<Xi>'; 
+    val_wa_foldnb_bod \<xi>\<^sub>m xs frm to (Fun (val.rename_expr rename' (val.monoexpr (specialise ts f))) [])
+         acc obsv res;
+\<forall>i<length xs. \<exists>v. xs ! i = VPrim (LU32 v);
+    \<Xi>, [], [option.Some Generated_TypeProof.abbreviatedType1] \<turnstile> App (Fun (val.rename_expr rename 
+      (val.monoexpr (specialise ts f))) []) (Var 0) : TPrim (Num U32)
+    \<rbrakk>
+       \<Longrightarrow> val_wa_foldnb_bod \<xi>\<^sub>p xs frm to (Fun f ts) acc obsv (VPrim (LU32 r))"
+  oops
 
 lemma val_wa_foldnb_0_mono_helper1:
   "\<lbrakk>val.proc_env_matches \<xi>m1 \<Xi>; proc_ctx_wellformed \<Xi>; \<forall>i<length xs. \<exists>v. xs ! i = VPrim (LU32 v);
     \<Xi>, [], [option.Some Generated_TypeProof.abbreviatedType1] \<turnstile> App (Fun (val.rename_expr rename 
       (val.monoexpr (specialise ts f))) []) (Var 0) : TPrim (Num U32);
-    val_wa_foldnb_bod_0 \<xi>m xs frm to (Fun (val.rename_expr rename (val.monoexpr (specialise ts f))) [])
+    val_wa_foldnb_bod \<xi>m xs frm to (Fun (val.rename_expr rename (val.monoexpr (specialise ts f))) [])
          (VPrim (LU32 acc)) VUnit (VPrim (LU32 r))\<rbrakk>
-       \<Longrightarrow> val_wa_foldnb_bod_0 \<xi>p xs frm to (Fun f ts) (VPrim (LU32 acc)) VUnit (VPrim (LU32 r))"
+       \<Longrightarrow> val_wa_foldnb_bod \<xi>p xs frm to (Fun f ts) (VPrim (LU32 acc)) VUnit (VPrim (LU32 r))"
   apply (induct to arbitrary: r)
-   apply (erule val_wa_foldnb_bod_0.elims; clarsimp)
-   apply (subst val_wa_foldnb_bod_0.simps; clarsimp)
+   apply (erule val_wa_foldnb_bod.elims; clarsimp)
+   apply (subst val_wa_foldnb_bod.simps; clarsimp)
   apply clarsimp
   apply (case_tac "length xs < Suc to")
    apply (erule_tac x = r in meta_allE)
-   apply (drule val_wa_foldnb_bod_0_back_step'; simp)
-   apply (drule val_wa_foldnb_bod_0_to_geq_lenD)
+   apply (drule val_wa_foldnb_bod_back_step'; simp)
+   apply (drule val_wa_foldnb_bod_to_geq_lenD)
     apply linarith
-   apply (rule val_wa_foldnb_bod_0_to_geq_len; simp)
+   apply (rule val_wa_foldnb_bod_to_geq_len; simp)
   apply (clarsimp simp: not_less)
   apply (case_tac "frm \<ge> to")
-   apply (erule val_wa_foldnb_bod_0.elims; clarsimp split: if_splits)
-    apply (erule val_wa_foldnb_bod_0.elims; clarsimp)
-    apply (subst val_wa_foldnb_bod_0.simps; clarsimp)
-    apply (subst val_wa_foldnb_bod_0.simps; clarsimp)
+   apply (erule val_wa_foldnb_bod.elims; clarsimp split: if_splits)
+    apply (erule val_wa_foldnb_bod.elims; clarsimp)
+    apply (subst val_wa_foldnb_bod.simps; clarsimp)
+    apply (subst val_wa_foldnb_bod.simps; clarsimp)
     apply (drule_tac \<gamma> = "[VRecord [xs ! frm, VPrim (LU32 acc), VUnit]]" and
       \<Gamma> = "[option.Some abbreviatedType1]" and
       e = "App (Fun f ts) (Var 0)" and
@@ -472,12 +580,12 @@ lemma val_wa_foldnb_0_mono_helper1:
       apply (rule val.v_t_r_empty)
      apply (erule_tac x = frm in allE; clarsimp)
     apply (case_tac v; clarsimp)
-   apply (subst val_wa_foldnb_bod_0.simps; clarsimp)
+   apply (subst val_wa_foldnb_bod.simps; clarsimp)
   apply (clarsimp simp: not_le)
   apply (frule_tac x = to in spec)
   apply (erule impE, simp)
   apply (erule exE)
-  apply (drule val_wa_foldnb_bod_0_back_step; simp?)
+  apply (drule val_wa_foldnb_bod_back_step; simp?)
   apply clarsimp
   apply (subgoal_tac "\<exists>y. r' = VPrim (LU32 y)", clarsimp)
    apply (erule_tac x = y in meta_allE)
@@ -500,17 +608,17 @@ lemma val_wa_foldnb_0_mono_helper1:
      apply (rule val.v_t_unit)
     apply (rule val.v_t_r_empty)
    apply (case_tac va; clarsimp)
-   apply (drule_tac r' = "VPrim (LU32 r)" in val_wa_foldnb_bod_0_step; simp)
+   apply (drule_tac r' = "VPrim (LU32 r)" in val_wa_foldnb_bod_step; simp)
   apply (insert val_proc_env_matches_\<xi>m_\<Xi>)
   apply (clarsimp simp: abbreviatedType1_def)
-  apply (drule val_wa_foldnb_bod_0_preservation; simp?)
-     apply clarsimp
+  apply (drule val_wa_foldnb_bod_preservation; simp?)
+     apply (clarsimp simp: wa_abs_typing_v_def)
      apply (erule_tac x = i in allE; clarsimp)
      apply (rule val.v_t_prim'; clarsimp)
-    apply (rule val.v_t_prim'; clarsimp)
-   apply (rule val.v_t_unit)
+    apply (rule val.v_t_unit)
+   apply clarsimp
   apply (erule v_t_prim_tE)
-  apply (drule lit_type_ex_32[OF sym])
+  apply (drule lit_type_ex[OF sym])
   apply clarsimp
   done
 
@@ -518,25 +626,25 @@ lemma val_wa_foldnb_0_mono_helper2:
   "\<lbrakk>val.proc_env_matches \<xi>m1 \<Xi>; proc_ctx_wellformed \<Xi>; \<forall>i<length xs. \<exists>v. xs ! i = VPrim (LU32 v);
     \<Xi>, [], [option.Some Generated_TypeProof.abbreviatedType1] \<turnstile> App (AFun (rename (f, ts)) []) 
       (Var 0) : TPrim (Num U32);
-    val_wa_foldnb_bod_0 \<xi>m xs frm to (AFun (rename (f, ts)) [])
+    val_wa_foldnb_bod \<xi>m xs frm to (AFun (rename (f, ts)) [])
          (VPrim (LU32 acc)) VUnit (VPrim (LU32 r))\<rbrakk>
-       \<Longrightarrow> val_wa_foldnb_bod_0 \<xi>p xs frm to (AFun f ts) (VPrim (LU32 acc)) VUnit (VPrim (LU32 r))"
+       \<Longrightarrow> val_wa_foldnb_bod \<xi>p xs frm to (AFun f ts) (VPrim (LU32 acc)) VUnit (VPrim (LU32 r))"
   apply (induct to arbitrary: r)
-   apply (erule val_wa_foldnb_bod_0.elims; clarsimp)
-   apply (subst val_wa_foldnb_bod_0.simps; clarsimp)
+   apply (erule val_wa_foldnb_bod.elims; clarsimp)
+   apply (subst val_wa_foldnb_bod.simps; clarsimp)
   apply clarsimp
   apply (case_tac "length xs < Suc to")
    apply (erule_tac x = r in meta_allE)
-   apply (drule val_wa_foldnb_bod_0_back_step'; simp)
-   apply (drule val_wa_foldnb_bod_0_to_geq_lenD)
+   apply (drule val_wa_foldnb_bod_back_step'; simp)
+   apply (drule val_wa_foldnb_bod_to_geq_lenD)
     apply linarith
-   apply (rule val_wa_foldnb_bod_0_to_geq_len; simp)
+   apply (rule val_wa_foldnb_bod_to_geq_len; simp)
   apply (clarsimp simp: not_less)
   apply (case_tac "frm \<ge> to")
-   apply (erule val_wa_foldnb_bod_0.elims; clarsimp split: if_splits)
-    apply (erule val_wa_foldnb_bod_0.elims; clarsimp)
-    apply (subst val_wa_foldnb_bod_0.simps; clarsimp)
-    apply (subst val_wa_foldnb_bod_0.simps; clarsimp)
+   apply (erule val_wa_foldnb_bod.elims; clarsimp split: if_splits)
+    apply (erule val_wa_foldnb_bod.elims; clarsimp)
+    apply (subst val_wa_foldnb_bod.simps; clarsimp)
+    apply (subst val_wa_foldnb_bod.simps; clarsimp)
     apply (drule_tac \<gamma> = "[VRecord [xs ! frm, VPrim (LU32 acc), VUnit]]" and
       \<Gamma> = "[option.Some abbreviatedType1]" and
       e = "App (AFun f ts) (Var 0)" and
@@ -557,12 +665,12 @@ lemma val_wa_foldnb_0_mono_helper2:
       apply (rule val.v_t_r_empty)
      apply (erule_tac x = frm in allE; clarsimp)
     apply (case_tac v; clarsimp)
-   apply (subst val_wa_foldnb_bod_0.simps; clarsimp)
+   apply (subst val_wa_foldnb_bod.simps; clarsimp)
   apply (clarsimp simp: not_le)
   apply (frule_tac x = to in spec)
   apply (erule impE, simp)
   apply (erule exE)
-  apply (drule val_wa_foldnb_bod_0_back_step; simp?)
+  apply (drule val_wa_foldnb_bod_back_step; simp?)
   apply clarsimp
   apply (subgoal_tac "\<exists>y. r' = VPrim (LU32 y)", clarsimp)
    apply (erule_tac x = y in meta_allE)
@@ -585,17 +693,17 @@ lemma val_wa_foldnb_0_mono_helper2:
      apply (rule val.v_t_unit)
     apply (rule val.v_t_r_empty)
    apply (case_tac va; clarsimp)
-   apply (drule_tac r' = "VPrim (LU32 r)" in val_wa_foldnb_bod_0_step; simp)
+   apply (drule_tac r' = "VPrim (LU32 r)" in val_wa_foldnb_bod_step; simp)
   apply (insert val_proc_env_matches_\<xi>m_\<Xi>)
   apply (clarsimp simp: abbreviatedType1_def)
-  apply (drule val_wa_foldnb_bod_0_preservation; simp?)
-     apply clarsimp
+  apply (drule val_wa_foldnb_bod_preservation; simp?)
+     apply (clarsimp simp: wa_abs_typing_v_def)
      apply (erule_tac x = i in allE; clarsimp)
      apply (rule val.v_t_prim'; clarsimp)
-    apply (rule val.v_t_prim'; clarsimp)
-   apply (rule val.v_t_unit)
+    apply (rule val.v_t_unit)
+   apply clarsimp
   apply (erule v_t_prim_tE)
-  apply (drule lit_type_ex_32[OF sym])
+  apply (drule lit_type_ex[OF sym])
   apply clarsimp
   done
 
@@ -606,25 +714,22 @@ lemma value_sem_rename_mono_prog_rename_\<Xi>_\<xi>m1_\<xi>p1:
    apply (rule_tac x = v' in exI)
    apply (subst (asm) rename_def)
    apply (subst (asm) assoc_lookup.simps)+
-   apply (clarsimp split: if_split_asm simp: val_wa_length_def)
-   apply (case_tac v; clarsimp)
+   apply (clarsimp split: if_split_asm)
+  apply (clarsimp simp: val_wa_length_rename_monoexpr_correct)
+  apply (rule conjI)
+   apply clarsimp
+   apply (rule_tac x = v' in exI)
+   apply (subst (asm) rename_def)
+   apply (subst (asm) assoc_lookup.simps)+
+   apply (clarsimp split: if_split_asm)
+  apply (clarsimp simp: val_wa_get_rename_monoexpr_correct)
+  apply clarsimp
   apply (rule conjI; clarsimp)
    apply (rule_tac x = v' in exI)
    apply (subst (asm) rename_def)
    apply (subst (asm) assoc_lookup.simps)+
-   apply (clarsimp split: if_split_asm simp: val_wa_get_def)
-   apply (case_tac v; clarsimp)
-   apply (case_tac z; clarsimp)
-   apply (case_tac za; clarsimp)
-  apply (rule conjI; clarsimp)
-   apply (rule_tac x = v' in exI)
-   apply (subst (asm) rename_def)
-   apply (subst (asm) assoc_lookup.simps)+
-   apply (clarsimp split: if_split_asm simp: val_wa_put2_def)
-   apply (case_tac v; clarsimp)
-   apply (case_tac z; clarsimp)
-   apply (case_tac za; clarsimp)
-   apply (case_tac zb; clarsimp)
+   apply (clarsimp split: if_split_asm)
+   apply (clarsimp simp: val_wa_put2_rename_monoexpr_correct)
   apply (subst (asm) rename_def)
   apply (subst (asm) assoc_lookup.simps)+
   apply (clarsimp split: if_split_asm simp: val_wa_foldnb_0_def val_wa_foldnb_0p_def)
@@ -648,43 +753,36 @@ lemma val_proc_env_matches_\<xi>m1_\<Xi>:
   apply (subst (asm) \<Xi>_def)
   apply (subst (asm) assoc_lookup.simps)+
   apply (clarsimp split: if_split_asm)
-     apply (clarsimp simp: wordarray_get_0_type_def abbreviatedType3_def val_wa_get_def)
-     apply (erule val.v_t_recordE)
-     apply (erule val.v_t_r_consE; clarsimp)
-     apply (erule val.v_t_abstractE; clarsimp simp: wa_abs_typing_v_def)
-     apply (case_tac va; clarsimp)
-    apply (rule val.v_t_prim[where l = "(LU32 _)", simplified])
-   apply (clarsimp simp: wordarray_length_0_type_def val_wa_length_def)
-   apply (rule val.v_t_prim[where l = "(LU32 _)", simplified])
-  apply (clarsimp simp: wordarray_put2_0_type_def abbreviatedType2_def val_wa_put2_def)
-  apply (erule val.v_t_recordE)
-  apply (erule val.v_t_r_consE; clarsimp)
-  apply (erule val.v_t_abstractE)
-  apply (rule val.v_t_abstract; clarsimp)
-   apply (clarsimp simp: wa_abs_typing_v_def)
-   apply (case_tac val; clarsimp)
-   apply (erule_tac x = i in allE; clarsimp)
-   apply (case_tac "i = unat idx"; clarsimp)
-  apply (clarsimp simp: wordarray_fold_no_break_0_type_def val_wa_foldnb_0_def)
+    apply (clarsimp simp: wordarray_get_0_type_def abbreviatedType3_def)
+    apply (drule val_wa_get_preservation; simp?)
+   apply (clarsimp simp: wordarray_length_0_type_def)
+  apply (drule val_wa_length_preservation; simp?)
+  apply (clarsimp simp: wordarray_put2_0_type_def abbreviatedType2_def)
+  apply (drule val_wa_put2_preservation; simp?)
+  apply (clarsimp simp: wordarray_fold_no_break_0_type_def val_wa_foldnb_0_def) thm val_wa_foldnb_bod_preservation
   apply (erule val.v_t_recordE)
   apply (erule val.v_t_r_consE; clarsimp)+
-  apply (rule val.v_t_prim'; simp)
+  apply (erule val.v_t_abstractE; clarsimp)
+  apply (clarsimp simp: abbreviatedType1_def)
+  apply (drule val_wa_foldnb_bod_preservation[OF proc_ctx_wellformed_\<Xi> val_proc_env_matches_\<xi>m_\<Xi>]; simp?)
+  apply clarsimp
   done
 
-lemma upd_wa_foldnb_bod_0_pres_obsv:
-  "\<lbrakk>upd_wa_foldnb_bod_0 \<xi>\<^sub>u \<sigma> p frm to f acc (obsv, s) (\<sigma>', res); upd_val_rel \<Xi>' \<sigma> obsv obsv' t s {};
-    \<sigma> p = option.Some (UAbstract (UWA (TPrim (Num n)) len arr)); \<forall>i < len. \<exists>x. \<sigma> (arr + size_of_num_type n * i) = option.Some x\<rbrakk> 
+lemma upd_wa_foldnb_bod_pres_obsv:
+  "\<lbrakk>upd_wa_foldnb_bod \<xi>\<^sub>u \<sigma> p frm to f acc obsv (ra \<union> s) (\<sigma>', res); upd_val_rel \<Xi>' \<sigma> obsv obsv' t s {};
+    \<sigma> p = option.Some (UAbstract (UWA (TPrim (Num n)) len arr)); 
+    \<forall>i < len. \<exists>x. \<sigma> (arr + size_of_num_type n * i) = option.Some x\<rbrakk> 
     \<Longrightarrow> upd_val_rel \<Xi>' \<sigma>' obsv obsv' t s {}"
   apply (induct to arbitrary: \<sigma>' res)
-   apply (erule upd_wa_foldnb_bod_0.elims; clarsimp)
+   apply (erule upd_wa_foldnb_bod.elims; clarsimp)
   apply (case_tac "len < 1 + to")
-   apply (drule upd_wa_foldnb_bod_0_back_step'; simp?)
+   apply (drule upd_wa_foldnb_bod_back_step'; simp?)
   apply (case_tac "frm < to")
    apply (frule_tac x = to in spec)
    apply (erule impE)
     apply (drule unatSuc; clarsimp simp: word_less_nat_alt)
    apply clarsimp
-   apply (drule upd_wa_foldnb_bod_0_back_step; simp?)
+   apply (drule upd_wa_foldnb_bod_back_step; simp?)
     apply (drule unatSuc; clarsimp simp: word_less_nat_alt)
    apply clarsimp
    apply (drule_tac x = \<sigma>'' in meta_spec)
@@ -693,53 +791,54 @@ lemma upd_wa_foldnb_bod_0_pres_obsv:
    apply (drule_tac upd_val_rel_frame(1); simp?)
    apply blast
   apply (case_tac "\<not> frm < 1 + to")
-   apply (erule upd_wa_foldnb_bod_0.elims; clarsimp)
+   apply (erule upd_wa_foldnb_bod.elims; clarsimp)
   apply (clarsimp simp: not_le not_less)
   apply (subgoal_tac "to = frm")
-  apply (erule upd_wa_foldnb_bod_0.elims; clarsimp split: if_splits)
-   apply (erule upd_wa_foldnb_bod_0.elims; clarsimp simp: add.commute)
+  apply (erule upd_wa_foldnb_bod.elims; clarsimp split: if_splits)
+   apply (erule upd_wa_foldnb_bod.elims; clarsimp simp: add.commute)
    apply (drule_tac upd_val_rel_frame(1); simp?)
    apply blast
   by (metis add.commute inc_le not_less word_le_less_eq)
 
-lemma upd_val_wa_foldnb_bod_0_corres:
-  "\<lbrakk>upd_wa_foldnb_bod_0 \<xi>\<^sub>u \<sigma> p frm to f acc (obsv, s) (\<sigma>', res); 
-    val_wa_foldnb_bod_0 \<xi>\<^sub>v xs (unat frm) (unat to) f acc' obsv' res';
+lemma upd_val_wa_foldnb_bod_corres:
+  "\<lbrakk>proc_ctx_wellformed \<Xi>'; proc_env_u_v_matches \<xi>\<^sub>u \<xi>\<^sub>v \<Xi>'; 
+    upd_wa_foldnb_bod \<xi>\<^sub>u \<sigma> p frm to f acc obsv (ra \<union> s) (\<sigma>', res); 
+    val_wa_foldnb_bod \<xi>\<^sub>v xs (unat frm) (unat to) f acc' obsv' res';
     \<sigma> p = option.Some (UAbstract (UWA v len arr));
     wa_abs_upd_val (UWA v len arr) (VWA v xs) ''WordArray'' [v] (Boxed ReadOnly undefined) r w \<sigma>;
-    upd_val_rel \<Xi>' \<sigma> acc acc' u ra wa; upd_val_rel \<Xi>' \<sigma> obsv obsv' t s {}; wa \<inter> s = {}; proc_ctx_wellformed \<Xi>';
+    upd_val_rel \<Xi>' \<sigma> acc acc' u ra wa; upd_val_rel \<Xi>' \<sigma> obsv obsv' t s {}; wa \<inter> s = {};
     \<tau> = TRecord [(''elem'', (v, Present)), (''acc'', (u, Present)), (''obsv'', (t, Present))] Unboxed;
-    proc_env_u_v_matches \<xi>\<^sub>u \<xi>\<^sub>v \<Xi>';  \<Xi>', [], [option.Some \<tau>] \<turnstile> App f (Var 0) : u\<rbrakk>
+     \<Xi>', [], [option.Some \<tau>] \<turnstile> App f (Var 0) : u\<rbrakk>
     \<Longrightarrow> \<exists>ra' wa'.  upd_val_rel \<Xi>' \<sigma>' res res' u ra' wa' \<and> ra' \<subseteq> ({p} \<union> ra \<union> s \<union> r)\<and> frame \<sigma> wa \<sigma>' wa'"
   apply (induct to arbitrary: res res' \<sigma>')
-   apply (erule upd_wa_foldnb_bod_0.elims; clarsimp)
-   apply (erule val_wa_foldnb_bod_0.elims; clarsimp)
+   apply (erule upd_wa_foldnb_bod.elims; clarsimp)
+   apply (erule val_wa_foldnb_bod.elims; clarsimp)
    apply (rule_tac x = ra in exI)
    apply (rule_tac x = wa in exI)
    apply (clarsimp simp: frame_def)
   apply (case_tac "len < 1 + to")
-   apply (drule upd_wa_foldnb_bod_0_back_step'; simp?)
+   apply (drule upd_wa_foldnb_bod_back_step'; simp?)
    apply (drule unatSuc; clarsimp)
-   apply (drule val_wa_foldnb_bod_0_back_step'; clarsimp simp: wa_abs_upd_val_def word_less_nat_alt)
+   apply (drule val_wa_foldnb_bod_back_step'; clarsimp simp: wa_abs_upd_val_def word_less_nat_alt)
    apply (case_tac v; clarsimp)
    apply (case_tac x5; clarsimp)
   apply (case_tac "1 + to \<le> frm")
    apply (frule_tac y = "1 + to" and x = frm in leD)
-   apply (erule upd_wa_foldnb_bod_0.elims; clarsimp)
+   apply (erule upd_wa_foldnb_bod.elims; clarsimp)
    apply (drule unatSuc; clarsimp simp: word_less_nat_alt word_le_nat_alt)
-   apply (erule val_wa_foldnb_bod_0.elims; clarsimp)
+   apply (erule val_wa_foldnb_bod.elims; clarsimp)
    apply (rule_tac x = ra in exI)
    apply (rule_tac x = wa in exI)
    apply (clarsimp simp: frame_def)
   apply (case_tac "frm = to")
    apply (clarsimp simp: not_le not_less)
-   apply (erule upd_wa_foldnb_bod_0.elims; clarsimp split: if_split_asm)
+   apply (erule upd_wa_foldnb_bod.elims; clarsimp split: if_split_asm)
    apply (erule disjE; clarsimp)
-    apply (erule upd_wa_foldnb_bod_0.elims; clarsimp simp: add.commute)
+    apply (erule upd_wa_foldnb_bod.elims; clarsimp simp: add.commute)
     apply (drule unatSuc; clarsimp simp: word_less_nat_alt word_le_nat_alt wa_abs_upd_val_def)
     apply (case_tac v; clarsimp)
-    apply (erule val_wa_foldnb_bod_0.elims; clarsimp)
-    apply (erule val_wa_foldnb_bod_0.elims; clarsimp)
+    apply (erule val_wa_foldnb_bod.elims; clarsimp)
+    apply (erule val_wa_foldnb_bod.elims; clarsimp)
     apply (erule_tac x = frm in allE; clarsimp)
     apply (frule_tac \<gamma> = "[URecord [(va, upd.uval_repr va), (acc, upd.uval_repr acc),
       (obsv, upd.uval_repr obsv)]]" and 
@@ -768,9 +867,9 @@ lemma upd_val_wa_foldnb_bod_0_corres:
    apply (erule impE)
     apply auto[1]
    apply clarsimp
-   apply (erule upd_wa_foldnb_bod_0.elims; clarsimp simp: add.commute)
+   apply (erule upd_wa_foldnb_bod.elims; clarsimp simp: add.commute)
     apply (drule unatSuc; clarsimp simp: word_less_nat_alt word_le_nat_alt wa_abs_upd_val_def)
-   apply (erule val_wa_foldnb_bod_0.elims; clarsimp)+
+   apply (erule val_wa_foldnb_bod.elims; clarsimp)+
    apply (frule_tac \<gamma> = "[URecord [(va, upd.uval_repr va), (acc, upd.uval_repr acc),
       (obsv, upd.uval_repr obsv)]]" and 
       \<gamma>' = "[VRecord [xs ! unat frm, acc', obsv']]" and
@@ -799,11 +898,11 @@ lemma upd_val_wa_foldnb_bod_0_corres:
   apply (clarsimp simp: wa_abs_upd_val_def)
   apply (case_tac v; clarsimp)
   apply (case_tac x5; clarsimp)
-  apply (drule upd_wa_foldnb_bod_0_back_step; simp?)
+  apply (drule upd_wa_foldnb_bod_back_step; simp?)
     apply (drule unatSuc; clarsimp simp: word_less_nat_alt)
    apply (metis add.commute inc_le not_less_iff_gr_or_eq)
   apply (drule unatSuc; clarsimp simp: word_less_nat_alt word_le_nat_alt)
-  apply (drule_tac val_wa_foldnb_bod_0_back_step; simp?)
+  apply (drule_tac val_wa_foldnb_bod_back_step; simp?)
    apply (meson Suc_leI not_less_iff_gr_or_eq word_less_nat_alt)
   apply clarsimp
   apply (drule_tac x = r'' in meta_spec)
@@ -822,25 +921,23 @@ lemma upd_val_wa_foldnb_bod_0_corres:
       apply (rule u_v_prim'; clarsimp)
      apply (rule u_v_r_cons1[where r' = s and w' = "{}", simplified]; simp?)
        apply (rule u_v_r_cons1[where r' = "{}" and w' = "{}", simplified]; simp?)
-         apply (drule upd_wa_foldnb_bod_0_pres_obsv; simp?)
-         apply clarsimp
-         apply (erule_tac x = i in allE)
-         apply (clarsimp simp: word_less_nat_alt)
+         apply (rule upd_val_rel_frame(1); simp?) 
+         apply (rule disjointI)
+         apply (thin_tac "frame _ _ _ _")
+         apply (clarsimp simp: frame_def)
+         apply (erule_tac x = y in allE)
+         apply (drule_tac x = y in orthD2; simp)
         apply (rule u_v_r_empty)
        apply (drule_tac u = obsv in upd_val_rel_to_uval_typing(1))
        apply (drule upd.type_repr_uval_repr(1); simp)
       apply (drule upd_val_rel_to_uval_typing(1))
       apply (thin_tac "frame _ _ _ _")
-      apply (case_tac "\<exists>e. e \<in> wa' \<inter> s"; simp)
-       apply (clarsimp simp: frame_def)
-       apply (erule_tac x = e in allE)+
-       apply clarsimp
-       apply (thin_tac "_ \<longrightarrow> _")
-       apply (erule impE)
-        apply (drule_tac x = e in orthD2; simp)
-       apply (drule upd_val_rel_to_uval_typing(1))
-       apply (drule_tac p = e and u = obsv in upd.uval_typing_valid(1)[rotated 1]; simp?)
-      apply blast
+      apply (rule disjointI)
+      apply (clarsimp simp: frame_def)
+      apply (erule_tac x = y in allE)+
+      apply clarsimp
+      apply (drule_tac x = y in orthD2; simp)
+      apply (drule_tac p = y and u = obsv in upd_val_rel_valid(1)[rotated 1]; simp?)
      apply (drule_tac u = r'' in upd_val_rel_to_uval_typing(1))
      apply (drule upd.type_repr_uval_repr(1); simp)
     apply (erule_tac x = to in allE; clarsimp)
@@ -856,41 +953,43 @@ lemma upd_val_wa_foldnb_bod_0_corres:
 
 
 
-lemma val_executes_from_upd_wa_foldnb_bod_0:
-  "\<lbrakk>upd_wa_foldnb_bod_0 \<xi>\<^sub>u \<sigma> p frm to f acc (obsv, s) (\<sigma>', res); \<sigma> p = option.Some (UAbstract (UWA v len arr));
+lemma val_executes_from_upd_wa_foldnb_bod:
+  "\<lbrakk>proc_ctx_wellformed \<Xi>'; proc_env_u_v_matches \<xi>\<^sub>u \<xi>\<^sub>v \<Xi>';
+    upd_wa_foldnb_bod \<xi>\<^sub>u \<sigma> p frm to f acc obsv (ra \<union> s) (\<sigma>', res);
+    \<sigma> p = option.Some (UAbstract (UWA v len arr));
     wa_abs_upd_val (UWA v len arr) (VWA v xs) ''WordArray'' [v] (Boxed ReadOnly undefined) r w \<sigma>;
-    upd_val_rel \<Xi>' \<sigma> acc acc' u ra wa; upd_val_rel \<Xi>' \<sigma> obsv obsv' t s {}; wa \<inter> s = {}; proc_ctx_wellformed \<Xi>';
+    upd_val_rel \<Xi>' \<sigma> acc acc' u ra wa; upd_val_rel \<Xi>' \<sigma> obsv obsv' t s {}; wa \<inter> s = {};
     \<tau> = TRecord [(''elem'', (v, Present)), (''acc'', (u, Present)), (''obsv'', (t, Present))] Unboxed;
-    proc_env_u_v_matches \<xi>\<^sub>u \<xi>\<^sub>v \<Xi>';  \<Xi>', [], [option.Some \<tau>] \<turnstile> App f (Var 0) : u\<rbrakk>
-    \<Longrightarrow> \<exists>res' r w. val_wa_foldnb_bod_0 \<xi>\<^sub>v xs (unat frm) (unat to) f acc' obsv' res' \<and> upd_val_rel \<Xi>' \<sigma>' res res' u r w"
+     \<Xi>', [], [option.Some \<tau>] \<turnstile> App f (Var 0) : u\<rbrakk>
+    \<Longrightarrow> \<exists>res' r w. val_wa_foldnb_bod \<xi>\<^sub>v xs (unat frm) (unat to) f acc' obsv' res' \<and> upd_val_rel \<Xi>' \<sigma>' res res' u r w"
   apply (induct arbitrary: \<sigma>' res rule: word_induct[where m = "to"])
-   apply (erule upd_wa_foldnb_bod_0.elims; clarsimp)
+   apply (erule upd_wa_foldnb_bod.elims; clarsimp)
    apply (rule_tac x = acc' in exI)
-   apply (subst val_wa_foldnb_bod_0.simps; clarsimp)
+   apply (subst val_wa_foldnb_bod.simps; clarsimp)
    apply (rule_tac x = ra in exI)
    apply (rule_tac x = wa in exI)
    apply clarsimp
   apply (case_tac "1 + n \<le> 0"; clarsimp)
-   apply (erule upd_wa_foldnb_bod_0.elims; clarsimp)
+   apply (erule upd_wa_foldnb_bod.elims; clarsimp)
    apply (rule_tac x = acc' in exI)
-   apply (subst val_wa_foldnb_bod_0.simps; clarsimp)
+   apply (subst val_wa_foldnb_bod.simps; clarsimp)
    apply (rule_tac x = ra in exI)
    apply (rule_tac x = wa in exI)
    apply clarsimp
   apply (case_tac "len < 1 + n")
-   apply (drule upd_wa_foldnb_bod_0_back_step'; simp?)
+   apply (drule upd_wa_foldnb_bod_back_step'; simp?)
    apply (erule_tac x = \<sigma>' in meta_allE)
    apply (erule_tac x = res in meta_allE)
    apply clarsimp
    apply (rule_tac x = res' in exI)
-   apply (drule val_wa_foldnb_bod_0_to_geq_lenD)
+   apply (drule val_wa_foldnb_bod_to_geq_lenD)
     apply (clarsimp simp: wa_abs_upd_val_def)
     apply (case_tac v; clarsimp)
     apply (case_tac x5; clarsimp)
     apply (simp add: unatSuc word_less_nat_alt)
    apply (drule unatSuc; clarsimp)
    apply (rule conjI)
-    apply (rule val_wa_foldnb_bod_0_to_geq_len; simp?)
+    apply (rule val_wa_foldnb_bod_to_geq_len; simp?)
     apply (clarsimp simp: wa_abs_upd_val_def)
     apply (case_tac v; clarsimp)
     apply (case_tac x5; clarsimp simp: word_less_nat_alt)
@@ -900,17 +999,17 @@ lemma val_executes_from_upd_wa_foldnb_bod_0:
   apply (case_tac "1 + n \<le> frm")
    apply (rule_tac x = acc' in exI)
   apply (frule_tac y = "1 + n" and x = frm in leD)
-   apply (erule upd_wa_foldnb_bod_0.elims; clarsimp)
+   apply (erule upd_wa_foldnb_bod.elims; clarsimp)
    apply (drule unatSuc; clarsimp simp: word_less_nat_alt word_le_nat_alt)
-   apply (subst val_wa_foldnb_bod_0.simps; clarsimp)
+   apply (subst val_wa_foldnb_bod.simps; clarsimp)
    apply (rule_tac x = ra in exI)
    apply (rule_tac x = wa in exI)
    apply clarsimp
   apply (case_tac "frm = n")
    apply (clarsimp simp: not_le not_less)
-   apply (erule upd_wa_foldnb_bod_0.elims; clarsimp split: if_split_asm)
+   apply (erule upd_wa_foldnb_bod.elims; clarsimp split: if_split_asm)
    apply (erule disjE; clarsimp)
-    apply (erule upd_wa_foldnb_bod_0.elims; clarsimp simp: add.commute)
+    apply (erule upd_wa_foldnb_bod.elims; clarsimp simp: add.commute)
     apply (frule_tac \<gamma> = "[URecord [(va, upd.uval_repr va), (acc, upd.uval_repr acc), 
       (obsv, upd.uval_repr obsv)]]" and 
       \<gamma>' = "[VRecord [xs ! unat frm, acc', obsv']]" and
@@ -935,8 +1034,8 @@ lemma val_executes_from_upd_wa_foldnb_bod_0:
     apply (rule_tac x = v' in exI)
     apply (drule unatSuc; clarsimp simp: word_less_nat_alt word_le_nat_alt)
     apply (rule conjI)
-     apply (subst val_wa_foldnb_bod_0.simps; clarsimp)
-     apply (subst val_wa_foldnb_bod_0.simps; clarsimp)
+     apply (subst val_wa_foldnb_bod.simps; clarsimp)
+     apply (subst val_wa_foldnb_bod.simps; clarsimp)
      apply (rule FalseE)
      apply (clarsimp simp: wa_abs_upd_val_def)
     apply (frule_tac \<gamma> = "[URecord [(va, upd.uval_repr va), (acc, upd.uval_repr acc),
@@ -952,7 +1051,7 @@ lemma val_executes_from_upd_wa_foldnb_bod_0:
        apply (rule u_v_r_cons1[where r' = s and w' = "{}", simplified]; simp?)
         apply (rule u_v_r_cons1[where r' = "{}" and w' = "{}", simplified]; simp?)
          apply (rule u_v_r_empty)
-        apply (drule_tac u = obsv in  upd_val_rel_to_uval_typing(1))
+        apply (drule_tac u = obsv in upd_val_rel_to_uval_typing(1))
         apply (drule upd.type_repr_uval_repr(1); simp)
        apply (drule upd_val_rel_to_uval_typing(1))
        apply (drule upd.type_repr_uval_repr(1); simp)
@@ -966,7 +1065,7 @@ lemma val_executes_from_upd_wa_foldnb_bod_0:
    apply (erule impE)
     apply simp
    apply clarsimp
-   apply (erule upd_wa_foldnb_bod_0.elims; clarsimp simp: add.commute)
+   apply (erule upd_wa_foldnb_bod.elims; clarsimp simp: add.commute)
    apply (drule unatSuc; clarsimp simp: word_less_nat_alt word_le_nat_alt)
    apply (frule_tac \<gamma> = "[URecord [(va, upd.uval_repr va), (acc, upd.uval_repr acc), 
       (obsv, upd.uval_repr obsv)]]" and
@@ -1012,21 +1111,21 @@ lemma val_executes_from_upd_wa_foldnb_bod_0:
    apply clarsimp
    apply (clarsimp simp: wa_abs_upd_val_def)
    apply (rule_tac x = v' in exI)
-   apply (subst val_wa_foldnb_bod_0.simps; clarsimp)+
+   apply (subst val_wa_foldnb_bod.simps; clarsimp)+
    apply (rule_tac x = r' in exI)
    apply (rule_tac x = w' in exI)
    apply clarsimp
   apply (clarsimp simp: wa_abs_upd_val_def)
   apply (case_tac v; clarsimp)
   apply (case_tac x5; clarsimp)
-  apply (drule_tac upd_wa_foldnb_bod_0_back_step; simp?)
+  apply (drule_tac upd_wa_foldnb_bod_back_step; simp?)
     apply (metis word_le_less_eq word_zero_le)
    apply (metis add.commute plus_one_helper word_le_less_eq word_not_le)
    apply clarsimp
    apply (drule_tac x = \<sigma>'' in meta_spec)
    apply (drule_tac x = r'' in meta_spec)
    apply clarsimp
-  apply (frule_tac r = r and w = w in upd_val_wa_foldnb_bod_0_corres; simp?)
+  apply (frule_tac r = r and w = w in upd_val_wa_foldnb_bod_corres; simp?)
    apply (clarsimp simp: wa_abs_upd_val_def)
   apply clarsimp
   apply (drule unatSuc; clarsimp simp: word_less_nat_alt word_le_nat_alt)
@@ -1041,9 +1140,12 @@ lemma val_executes_from_upd_wa_foldnb_bod_0:
       apply (rule u_v_prim'; clarsimp)
      apply (rule u_v_r_cons1[where r' = s and w' = "{}", simplified]; simp?)
        apply (rule u_v_r_cons1[where r' = "{}" and w' = "{}", simplified]; simp?)
-         apply (drule upd_wa_foldnb_bod_0_pres_obsv; simp?)
-         apply clarsimp
-         apply (erule_tac x = i in allE; clarsimp simp: word_less_nat_alt)+
+         apply (rule upd_val_rel_frame(1); simp?)
+         apply (rule disjointI)
+         apply (thin_tac "frame _ _ _ _")
+         apply (clarsimp simp: frame_def)
+         apply (erule_tac x = y in allE)
+         apply (drule_tac x = y in orthD2; simp)
         apply (rule u_v_r_empty)
        apply (drule_tac u = obsv in  upd_val_rel_to_uval_typing(1))
        apply (drule upd.type_repr_uval_repr(1); simp)
@@ -1052,14 +1154,13 @@ lemma val_executes_from_upd_wa_foldnb_bod_0:
       apply (clarsimp simp: frame_def)
       apply (erule_tac x = y in allE; clarsimp)+
       apply (drule_tac x = y in orthD2; simp)
-      apply (drule_tac u = obsv and p = y in upd_val_rel_valid(1)[where r = s and w = "{}", simplified]; simp?)
-      apply clarsimp
+      apply (drule_tac u = obsv and p = y in upd_val_rel_valid(1)[rotated 1]; simp?)
      apply (drule_tac u = r'' in  upd_val_rel_to_uval_typing(1))
      apply (drule upd.type_repr_uval_repr(1); simp)
     apply (erule_tac x = n in allE; clarsimp)+
    apply (rule u_v_matches_empty[where \<tau>s = "[]", simplified])
   apply clarsimp
-  apply (drule_tac r' = v' in  val_wa_foldnb_bod_0_step; simp?)
+  apply (drule_tac r' = v' in  val_wa_foldnb_bod_step; simp?)
   apply (rule_tac x = v' in exI)
   apply clarsimp
   apply (frule_tac \<gamma> = "[URecord [(va, upd.uval_repr va), (r'', upd.uval_repr r''), 
@@ -1073,9 +1174,12 @@ lemma val_executes_from_upd_wa_foldnb_bod_0:
       apply (rule u_v_prim'; clarsimp)
      apply (rule u_v_r_cons1[where r' = s and w' = "{}", simplified]; simp?)
        apply (rule u_v_r_cons1[where r' = "{}" and w' = "{}", simplified]; simp?)
-         apply (drule upd_wa_foldnb_bod_0_pres_obsv; simp?)
-         apply clarsimp
-         apply (erule_tac x = i in allE; clarsimp simp: word_less_nat_alt)
+         apply (rule upd_val_rel_frame(1); simp?) 
+         apply (rule disjointI)
+         apply (thin_tac "frame _ _ _ _")
+         apply (clarsimp simp: frame_def)
+         apply (erule_tac x = y in allE)
+         apply (drule_tac x = y in orthD2; simp)
         apply (rule u_v_r_empty)
        apply (drule_tac u = obsv in  upd_val_rel_to_uval_typing(1))
        apply (drule upd.type_repr_uval_repr(1); simp)
@@ -1084,8 +1188,7 @@ lemma val_executes_from_upd_wa_foldnb_bod_0:
       apply (clarsimp simp: frame_def)
       apply (erule_tac x = y in allE; clarsimp)+
       apply (drule_tac x = y in orthD2; simp)
-      apply (drule_tac u = obsv and p = y in upd_val_rel_valid(1)[where r = s and w = "{}", simplified]; simp?)
-      apply clarsimp
+      apply (drule_tac u = obsv and p = y in upd_val_rel_valid(1)[rotated 1]; simp?)
      apply (drule_tac u = r'' in  upd_val_rel_to_uval_typing(1))
      apply (drule upd.type_repr_uval_repr(1); simp)
     apply (erule_tac x = n in allE; clarsimp)
@@ -1108,51 +1211,31 @@ lemma wordarray_fold_no_break_upd_val:
   apply (erule u_v_p_absE'; clarsimp)
   apply (erule u_v_r_consE'; simp)
   apply (erule conjE)+
-  apply (drule_tac t = ts in sym)
-  apply (drule_tac t = t in sym)
-  apply (drule_tac t = "type_repr t" in sym)
-  apply (drule_tac t = xa in sym)
-  apply (drule_tac t = n in sym)
+  apply (drule_tac t = "type_repr _" in sym)
   apply clarsimp
   apply (erule u_v_primE')
-  apply (drule_tac s = "Num U32" in sym)
+  apply (drule_tac t = "lit_type _" in sym)
   apply clarsimp
   apply (erule u_v_r_consE'; simp)
   apply (erule conjE)+
-  apply (drule_tac t = ts in sym)
-  apply (drule_tac t = t in sym)
-  apply (drule_tac t = "type_repr t" in sym)
-  apply (drule_tac t = xa in sym)
-  apply (drule_tac t = n in sym)
+  apply (drule_tac t = "type_repr _" in sym)
   apply clarsimp
   apply (erule u_v_primE')
-  apply (drule_tac s = "Num U32" in sym)
+  apply (drule_tac t = "lit_type _" in sym)
   apply clarsimp
   apply (erule u_v_r_consE'; simp)
   apply (erule conjE)+
-  apply (drule_tac t = ts in sym)
-  apply (drule_tac t = t in sym)
-  apply (drule_tac t = "type_repr t" in sym)
-  apply (drule_tac t = xa in sym)
-  apply (drule_tac t = n in sym)
+  apply (drule_tac t = "type_repr _" in sym)
   apply clarsimp
   apply (erule u_v_r_consE'; simp)
   apply (erule conjE)+
-  apply (drule_tac t = ts in sym)
-  apply (drule_tac t = t in sym)
-  apply (drule_tac t = "type_repr t" in sym)
-  apply (drule_tac t = xa in sym)
-  apply (drule_tac t = n in sym)
+  apply (drule_tac t = "type_repr _" in sym)
   apply clarsimp
   apply (erule u_v_primE')
-  apply (drule_tac s = "Num U32" in sym)
+  apply (drule_tac t = "lit_type _" in sym)
   apply clarsimp
   apply (erule u_v_r_consE'; simp)
   apply (erule conjE)+
-  apply (drule_tac t = ts in sym)
-  apply (drule_tac t = t in sym)
-  apply (drule_tac t = xa in sym)
-  apply (drule_tac t = n in sym)
   apply clarsimp
   apply (erule u_v_r_emptyE'; clarsimp)
   apply (subst (asm) upd_val_rel.simps[of _ _ "UUnit", simplified])
@@ -1162,87 +1245,69 @@ lemma wordarray_fold_no_break_upd_val:
   apply (case_tac a'; clarsimp simp: wa_abs_upd_val_def val_wa_foldnb_0_def)
   apply (case_tac x11; clarsimp)
   apply (case_tac x5; clarsimp)
-  apply (case_tac x; clarsimp)
+  apply (rule conjI; clarsimp)
+   apply (drule_tac xs = x12 and r = r and w = "{}" and acc' = "VPrim (LU32 acc)" and 
+      wa = "{}" and obsv' = "VUnit" and t = "TUnit" and res' = "(VPrim (LU32 rc))"
+      in upd_val_wa_foldnb_bod_corres[OF proc_ctx_wellformed_\<Xi> proc_env_u_v_matches_\<xi>0_\<xi>m_\<Xi>,
+        where ra = "{}" and s = "{}", simplified]; simp?)
+        apply (case_tac xa; clarsimp)
+         apply (subst (asm) upd_val_rel.simps[of _ _ "UFunction _ _", simplified])
+         apply clarsimp
+         apply (erule disjE; clarsimp?)
+         apply (erule disjE; clarsimp?)
+        apply (subst (asm) upd_val_rel.simps[of _ _ "UAFunction _ _", simplified])
+        apply clarsimp
+        apply (erule disjE; clarsimp?)
+        apply (erule disjE; clarsimp?)
+       apply (clarsimp simp: wa_abs_upd_val_def)
+      apply (rule u_v_prim'; clarsimp)
+     apply (rule u_v_unit)
+    apply (clarsimp simp: abbreviatedType1_def)
+   apply clarsimp
+   apply (case_tac xa; clarsimp)
+    apply (subst (asm) upd_val_rel.simps[of _ _ "UFunction _ _", simplified])
+    apply clarsimp
+    apply (erule disjE; clarsimp?)
+    apply (erule disjE; clarsimp?)
+    apply blast
+   apply (subst (asm) upd_val_rel.simps[of _ _ "UAFunction _ _", simplified])
+   apply clarsimp
+   apply (erule disjE; clarsimp?)
+   apply (erule disjE; clarsimp?)
+   apply blast
+  apply (drule_tac xs = x12 and r = r and w = "{}" and acc' = "VPrim (LU32 acc)" and
+      wa = "{}" and obsv' = "VUnit" and t = "TUnit" 
+      in val_executes_from_upd_wa_foldnb_bod[OF proc_ctx_wellformed_\<Xi> proc_env_u_v_matches_\<xi>0_\<xi>m_\<Xi>,
+        where ra = "{}" and s = "{}", simplified]; simp?)
+      apply (clarsimp simp: wa_abs_upd_val_def)
+     apply (rule u_v_prim'; clarsimp)
+    apply (rule u_v_unit)
+   apply (clarsimp simp: abbreviatedType1_def)
+  apply clarsimp
+  apply (rule_tac x = res' in exI)
+  apply (clarsimp simp: val_wa_foldnb_0_def)
+  apply (rule conjI)
+  apply (clarsimp simp: abbreviatedType1_def)
+  apply (drule val_wa_foldnb_bod_preservation[OF proc_ctx_wellformed_\<Xi> val_proc_env_matches_\<xi>m_\<Xi>]; simp?)
+      apply (clarsimp simp: wa_abs_typing_v_def)
+      apply (rule val.v_t_prim'; simp)
+     apply (rule val.v_t_unit)
+    apply clarsimp
+   apply (erule v_t_prim_tE; clarsimp) 
+   apply (drule lit_type_ex[OF sym]; simp)
+  apply (rule conjI, clarsimp simp: wa_abs_typing_v_def)
+   apply (erule_tac x = i in allE; clarsimp)
+   apply (drule lit_type_ex; simp)
+  apply (case_tac xa; clarsimp)
    apply (subst (asm) upd_val_rel.simps[of _ _ "UFunction _ _", simplified])
    apply clarsimp
    apply (erule disjE; clarsimp?)
    apply (erule disjE; clarsimp?)
-   apply (rule conjI; clarsimp)
-    apply (drule_tac xs = x12 and r = r and w = "{}" and acc' = "VPrim (LU32 acc)" and
-      ra = "{}" and wa = "{}" and obsv' = "VUnit" and t = "TUnit"
-      in upd_val_wa_foldnb_bod_0_corres; simp?)
-         apply (clarsimp simp: wa_abs_upd_val_def)
-        apply (rule u_v_prim'; clarsimp)
-       apply (rule u_v_unit)
-      apply (rule proc_ctx_wellformed_\<Xi>)
-     apply (clarsimp simp: abbreviatedType1_def)
-    apply (rule proc_env_u_v_matches_\<xi>0_\<xi>m_\<Xi>)
-   apply (drule_tac xs = x12 and r = r and w = "{}" and acc' = "VPrim (LU32 acc)" and
-      ra = "{}" and wa = "{}" and obsv' = "VUnit" and t = "TUnit" 
-      in val_executes_from_upd_wa_foldnb_bod_0; simp?)
-         apply (clarsimp simp: wa_abs_upd_val_def wa_abs_typing_v_def)
-        apply (rule u_v_prim'; clarsimp)
-       apply (rule u_v_unit)
-      apply (rule proc_ctx_wellformed_\<Xi>)
-     apply (clarsimp simp: abbreviatedType1_def)
-    apply (rule proc_env_u_v_matches_\<xi>0_\<xi>m_\<Xi>)
-   apply clarsimp
-   apply (rule_tac x = res' in exI)
-   apply (clarsimp simp: val_wa_foldnb_0_def)
-   apply (clarsimp simp: abbreviatedType1_def)
-   apply (rule conjI)
-    apply (clarsimp simp: wa_abs_typing_v_def)
-    apply (drule val_wa_foldnb_bod_0_preservation[OF proc_ctx_wellformed_\<Xi> val_proc_env_matches_\<xi>m_\<Xi>]; simp?)
-       apply (clarsimp simp: wa_abs_typing_v_def)
-       apply (erule_tac x = i in allE; clarsimp)+
-      apply (rule val.v_t_prim'; simp)
-     apply (rule val.v_t_prim'; simp)
-    apply (rule val.v_t_unit)
-   apply (erule v_t_prim_tE; clarsimp)
-    apply (drule lit_type_ex_32[OF sym]; simp)
-   apply (clarsimp simp: wa_abs_typing_v_def)
-   apply (erule_tac x = i in allE; clarsimp)
-   apply (drule lit_type_ex_32; simp)
   apply (subst (asm) upd_val_rel.simps[of _ _ "UAFunction _ _", simplified])
   apply clarsimp
   apply (erule disjE; clarsimp?)
   apply (erule disjE; clarsimp?)
-  apply (rule conjI; clarsimp)
-   apply (drule_tac xs = x12 and r = r and w = "{}" and acc' = "VPrim (LU32 acc)" and
-      ra = "{}" and wa = "{}" and obsv' = "VUnit" and t = "TUnit" 
-      in upd_val_wa_foldnb_bod_0_corres; simp?)
-        apply (clarsimp simp: wa_abs_upd_val_def)
-       apply (rule u_v_prim'; clarsimp)
-      apply (rule u_v_unit)
-     apply (rule proc_ctx_wellformed_\<Xi>)
-    apply (clarsimp simp: abbreviatedType1_def)
-   apply (rule proc_env_u_v_matches_\<xi>0_\<xi>m_\<Xi>)
-  apply (drule_tac xs = x12 and r = r and w = "{}" and acc' = "VPrim (LU32 acc)" and
-      ra = "{}" and wa = "{}" and obsv' = "VUnit" and t = "TUnit" 
-      in val_executes_from_upd_wa_foldnb_bod_0; simp?)
-        apply (clarsimp simp: wa_abs_upd_val_def wa_abs_typing_v_def)
-       apply (rule u_v_prim'; clarsimp)
-      apply (rule u_v_unit)
-     apply (rule proc_ctx_wellformed_\<Xi>)
-    apply (clarsimp simp: abbreviatedType1_def)
-   apply (rule proc_env_u_v_matches_\<xi>0_\<xi>m_\<Xi>)
-  apply clarsimp
-  apply (rule_tac x = res' in exI)
-  apply (clarsimp simp: val_wa_foldnb_0_def wa_abs_typing_v_def)
-  apply (clarsimp simp: abbreviatedType1_def)
-  apply (drule val_wa_foldnb_bod_0_preservation[OF proc_ctx_wellformed_\<Xi> val_proc_env_matches_\<xi>m_\<Xi>]; simp?)
-     apply clarsimp
-     apply (erule_tac x = i in allE; clarsimp)+
-     apply (rule val.v_t_prim'; simp)
-    apply (rule val.v_t_prim'; simp)
-   apply (rule val.v_t_unit)
-  apply (erule v_t_prim_tE; clarsimp)
-  apply (drule lit_type_ex_32[OF sym]; simp)
-  apply clarsimp
-  apply (erule_tac x = i in allE; clarsimp)
-  apply (drule lit_type_ex_32; simp)
   done
-
 
 lemma upd_proc_env_matches_ptrs_\<xi>1_\<Xi>:
   "upd.proc_env_matches_ptrs \<xi>1 \<Xi>"
@@ -1251,10 +1316,13 @@ lemma upd_proc_env_matches_ptrs_\<xi>1_\<Xi>:
   apply (subst (asm) \<Xi>_def)
   apply (subst (asm) assoc_lookup.simps)+
   apply (clarsimp split: if_split_asm)
-     apply (clarsimp simp: wordarray_get_uval_typing_frame)
-    apply (clarsimp simp: wordarray_length_uval_typing_frame)
-   apply (clarsimp simp: wordarray_put2_uval_typing_frame)
-  apply (clarsimp simp: wordarray_fold_no_break_uval_typing_frame)
+     apply (clarsimp simp: wordarray_get_0_type_def abbreviatedType3_def)
+     apply (drule upd_wa_get_preservation; simp?)
+    apply (clarsimp simp: wordarray_length_0_type_def)
+    apply (drule upd_wa_length_preservation; simp)
+   apply (clarsimp simp: wordarray_put2_0_type_def abbreviatedType2_def)
+   apply (drule upd_wa_put2_preservation; simp)
+  apply (clarsimp simp: upd_wa_foldnb_0_preservation)
   done
 
 lemma proc_env_u_v_matches_\<xi>1_\<xi>m1_\<Xi>:
@@ -1263,9 +1331,12 @@ lemma proc_env_u_v_matches_\<xi>1_\<xi>m1_\<Xi>:
   apply (subst (asm) \<Xi>_def)
   apply (subst (asm) assoc_lookup.simps)+
   apply (clarsimp split: if_split_asm)
-     apply (clarsimp simp: wordarray_get_upd_val)
-    apply (clarsimp simp: wordarray_length_upd_val)
-   apply (clarsimp simp: wordarray_put2_upd_val)
+     apply (clarsimp simp: wordarray_get_0_type_def abbreviatedType3_def)
+     apply (drule wa_get_upd_val; simp)
+    apply (clarsimp simp: wordarray_length_0_type_def)
+    apply (drule wa_length_upd_val; simp)
+   apply (clarsimp simp: wordarray_put2_0_type_def abbreviatedType2_def)
+   apply (drule wa_put2_upd_val; simp)
   apply (clarsimp simp: wordarray_fold_no_break_upd_val)
   done
 
@@ -1273,9 +1344,9 @@ lemma proc_env_u_v_matches_\<xi>1_\<xi>m1_\<Xi>:
 
 
 lemma 
-  "\<lbrakk>val_wa_foldnb_bod_0 xs frm (Suc to) f acc obsv r; frm < Suc to\<rbrakk>
-    \<Longrightarrow> \<exists>acc'. val_wa_foldnb_bod_0 xs to (Suc to) f acc' obsv r"
-  apply (induct rule: val_wa_foldnb_bod_0.induct[where ?a0.0 = xs and
+  "\<lbrakk>val_wa_foldnb_bod xs frm (Suc to) f acc obsv r; frm < Suc to\<rbrakk>
+    \<Longrightarrow> \<exists>acc'. val_wa_foldnb_bod xs to (Suc to) f acc' obsv r"
+  apply (induct rule: val_wa_foldnb_bod.induct[where ?a0.0 = xs and
                                                        ?a1.0 = frm and
                                                        ?a2.0 = to and
                                                        ?a3.0 = f and
@@ -1284,31 +1355,31 @@ lemma
                                                        ?a6.0 = r]; clarsimp)
   apply (case_tac "frm < length xs")
    apply (case_tac "frm < to")
-    apply (erule val_wa_foldnb_bod_0.elims; clarsimp)
+    apply (erule val_wa_foldnb_bod.elims; clarsimp)
    apply clarsimp
    apply (rule_tac x = acc in exI)
-   apply (erule val_wa_foldnb_bod_0.elims; clarsimp)+
-   apply (subst val_wa_foldnb_bod_0.simps; clarsimp)+
+   apply (erule val_wa_foldnb_bod.elims; clarsimp)+
+   apply (subst val_wa_foldnb_bod.simps; clarsimp)+
    apply (rule_tac x = v in exI)
    apply clarsimp
    apply (subgoal_tac "frma = to")
     apply clarsimp
    apply linarith
   apply (rule_tac x = res in exI)
-  apply (subst val_wa_foldnb_bod_0.simps; clarsimp)
+  apply (subst val_wa_foldnb_bod.simps; clarsimp)
   done
 lemma 
-  "\<lbrakk>val_wa_foldnb_bod_0 xs frm to f (VPrim (LU32 acc)) VUnit r; 
+  "\<lbrakk>val_wa_foldnb_bod xs frm to f (VPrim (LU32 acc)) VUnit r; 
     \<forall>i<length xs. \<exists>v. xs ! i = VPrim (LU32 v);
     \<Xi>, [], [option.Some abbreviatedType1] \<turnstile> App f (Var 0) : TPrim (Num U32)\<rbrakk>
     \<Longrightarrow> \<exists>x. r = VPrim (LU32 x)"
   apply (induct to arbitrary: r)
-   apply (erule val_wa_foldnb_bod_0.elims; clarsimp)
+   apply (erule val_wa_foldnb_bod.elims; clarsimp)
   apply (case_tac "length xs < Suc to")
-   apply (drule val_wa_foldnb_bod_0_back_step'; simp)
+   apply (drule val_wa_foldnb_bod_back_step'; simp)
   apply (case_tac "to \<le> frm")
-   apply (erule val_wa_foldnb_bod_0.elims; clarsimp split: if_splits)
-   apply (erule val_wa_foldnb_bod_0.elims; clarsimp)
+   apply (erule val_wa_foldnb_bod.elims; clarsimp split: if_splits)
+   apply (erule val_wa_foldnb_bod.elims; clarsimp)
    apply (insert proc_ctx_wellformed_\<Xi> val_proc_env_matches_\<xi>m_\<Xi>)
    apply (drule val.preservation(1)[of "[]" "[]" _ _ _  \<xi>m, simplified]; simp?)
     apply (clarsimp simp: abbreviatedType1_def)
@@ -1322,10 +1393,10 @@ lemma
     apply (rule val.v_t_r_cons1; clarsimp?)
      apply (rule val.v_t_unit)
     apply (rule val.v_t_r_empty)
-   apply (erule v_t_prim_tE; clarsimp simp: lit_type_ex_32)
+   apply (erule v_t_prim_tE; clarsimp simp: lit_type_ex)
   apply (clarsimp simp: not_less not_le)
   apply (erule_tac x = to in allE; clarsimp)
-  apply (drule val_wa_foldnb_bod_0_back_step; simp?)
+  apply (drule val_wa_foldnb_bod_back_step; simp?)
   apply clarsimp
   apply (drule_tac x = r' in meta_spec)
   apply clarsimp
@@ -1342,30 +1413,10 @@ lemma
    apply (rule val.v_t_r_cons1; clarsimp?)
     apply (rule val.v_t_unit)
    apply (rule val.v_t_r_empty)
-  apply (erule v_t_prim_tE; clarsimp simp: lit_type_ex_32)
+  apply (erule v_t_prim_tE; clarsimp simp: lit_type_ex)
   done
 
-
-  term fold
-function extract_ptr :: "(funtyp, abstyp, ptrtyp) uval \<Rightarrow> (funtyp, abstyp, ptrtyp) store \<Rightarrow> ptrtyp set \<Rightarrow> ptrtyp set"
-  where
-"extract_ptr (UPrim _) _ ps = ps" |
-"extract_ptr UUnit _ ps = ps" |
-"extract_ptr (UFunction _ _) _ ps = ps" |
-"extract_ptr (UAFunction _ _) _ ps = ps" |
-"extract_ptr (UAbstract _) _  ps = ps" |
-"extract_ptr (UProduct a b) \<sigma> ps = fold (\<lambda>x ps. extract_ptr x \<sigma> ps) [a, b] ps" |
-"extract_ptr (USum _ a _) \<sigma> ps = extract_ptr a \<sigma> ps" | 
-"extract_ptr (URecord fs) \<sigma> ps = fold (\<lambda>x ps. extract_ptr x \<sigma> ps) (map prod.fst fs) ps" |
-"extract_ptr (UPtr p _) \<sigma> ps = 
-  (if p \<in> ps \<or> p > max_word then ps 
-  else (case \<sigma> p of option.Some x \<Rightarrow> extract_ptr x \<sigma> (insert p ps)
-                    | _ \<Rightarrow> ps))"
-  by pat_completeness auto
-termination
-  oops
 *)
-
 
 end (* of context *)
 
